theories/crypto/NominalGroup.ec
@@ -7,7 +7,7 @@ import Ring.IntID StdOrder.IntOrder.
 
 (* -------------------------------------------------------------------- *)
 
-op injective_on (A : 'a fset) (f : 'a -> 'b) : bool = 
+op injective_on (A : 'a fset) (f : 'a -> 'b) : bool =
   forall (x y : 'a), x \in A => y \in A => f x = f y => x = y.
 
 abstract theory NominalGroup.
@@ -27,7 +27,7 @@ op ( * ) : Z -> Z -> Z.
 op inv   : Z -> Z.
 
 op f : Z.
-op exp(a,x) = a^(x*inv f).
+op exp (a, x) = a ^ (x * inv f).
 
 op EU : Z fset.
 op dZ : Z distr.
@@ -35,28 +35,31 @@ op dZ : Z distr.
 axiom mulA       : associative ( * ).
 axiom mulC       : commutative ( * ).
 
-axiom expM       : forall a x y, a^(x * y) = (a^x)^y. 
-axiom exp_inv    : forall x, x \in EU => g^(x * inv x) = g.
-axiom exp_inv_f  : forall a, a^(f * inv f) = a.
+axiom powM       : forall a x y, a ^ (x * y) = (a ^ x) ^ y.
+axiom pow_inv    : forall x, x \in EU => g ^ (x * inv x) = g.
+axiom pow_inv_f  : forall a, a ^ (f * inv f) = a.
 
-axiom exp_inj    : injective_on EU(exp g).
-axiom exp_inj'   : forall x, injective_on EU(fun z => exp g (x*z)).
+axiom exp_inj    : injective_on EU (exp g).
+axiom exp_inj'   : forall x, injective_on EU (fun z => exp g (x * z)).
 
-axiom img_exp    : forall x, x \in EU => image (fun z => exp g (x*z)) EU = image (exp g) EU.
+axiom img_exp    : forall x, x \in EU =>
+                             image (fun z => exp g (x * z)) EU =
+                             image (exp g) EU.
 
+(* to remove *)
 axiom Emult x y  : x \in EU => y \in EU => x * y \in EU.
-axiom Einv x     : x \in EU => inv x \in EU. 
+axiom Einv x     : x \in EU => inv x \in EU.
 
 lemma invK a x   : a \in EU => x \in EU => a * x * inv x = a.
-proof. 
-move => aE bE; apply: exp_inj => //; last smt(expM exp_inv mulA mulC).
-apply: Emult => //. apply: Emult => //. exact: Einv.
+proof.
+move => aE bE; apply: exp_inj => //; last smt(mulA mulC powM pow_inv).
+apply: Emult => //; [by apply: Emult | by exact: Einv].
 qed.
 
 lemma invK' a x   : a \in EU => x \in EU => a * inv x * x = a.
-proof. rewrite -mulA (mulC _ x) mulA. exact: invK. qed.
+proof. by rewrite -mulA (mulC _ x) mulA; exact: invK. qed.
 
-lemma expM' a x y : exp a (x * y) = (exp a x)^y.
-proof. by rewrite /exp -!expM -!mulA (mulC y). qed.
+lemma expM a x y : exp a (x * y) = (exp a x) ^ y.
+proof. by rewrite /exp -!powM -!mulA (mulC y). qed.
 
 end NominalGroup.
